trying some proofs: get_addl/subl and memory_region_start_addr

codeTest/test_getMemRegion_start_addr.v
@@ -1,5 +1,5 @@
 Require Import generated.
-From dx.tests Require Import ChkPrimitive DxIntegers DxValues DxState DxMonad DxInstructions.
+From dx.tests Require Import ChkPrimitive DxIntegers DxValues DxMemRegion DxState DxMonad DxInstructions.
 From dx Require Import ResultMonad IR.
 From Coq Require Import List.
 From compcert Require Import Values Clight Memory.
@@ -8,37 +8,41 @@ Require Import ZArith.
 
 Definition val64_correct (x :val) (m: Memory.Mem.mem) (v:val) := x = v /\ exists v', Vlong v' = v.
 
-Definition args_binary_val64_correct : DList.t (fun x => coqType x -> Memory.Mem.mem -> val -> Prop) (compilableSymbolArgTypes val64Toval64Toval64SymbolType) :=
-  @DList.DCons _ _ val64CompilableType val64_correct _
-               (@DList.DCons _  _
-                             val64CompilableType val64_correct _
-                             (@DList.DNil CompilableType _)).
+Definition start_addr_correct (x :memory_region) (m: Memory.Mem.mem) (v:val) := exists b ofs v', (v = Vptr b ofs) /\ (Mem.loadv AST.Mint64 m v = Some (start_addr x)) /\ Vlong v' = start_addr x.
+
+Definition args_start_addr_correct : DList.t (fun x => coqType x -> Memory.Mem.mem -> val -> Prop) (compilableSymbolArgTypes mem_regionToVal64CompilableSymbolType) :=
+  @DList.DCons _  _
+                             mem_regionCompilableType start_addr_correct _
+                             (@DList.DNil CompilableType _).
+
+Section GetMemRegion_start_addr.
 
 (** The program contains our function of interest [fn] *)
 Definition p : Clight.program := prog.
 
 (* [Args,Res] provides the mapping between the Coq and the C types *)
-Definition Args : list CompilableType := [val64CompilableType; val64CompilableType].
+Definition Args : list CompilableType := [mem_regionCompilableType].
 Definition Res : CompilableType := val64CompilableType.
 
 (* [f] is a Coq Monadic function with the right type *)
-Definition f : encodeCompilableSymbolType (Some M) (MkCompilableSymbolType Args (Some Res)) := get_addl.
+Definition f : encodeCompilableSymbolType (Some M) (MkCompilableSymbolType Args (Some Res)) := getMemRegion_start_addr.
 
 (* [fn] is the Cligth function which has the same behaviour as [f] *)
-Definition fn: Clight.function := f_get_addl.
+Definition fn: Clight.function := f_getMemRegion_start_addr.
 
 (* [match_mem] related the Coq monadic state and the C memory *)
-Definition match_mem : stateM -> genv -> Memory.Mem.mem -> Prop :=
+Definition match_mem : stateM -> genv -> Mem.mem -> Prop :=
   fun stm g m =>
     g = globalenv p /\
       (match Globalenvs.Genv.alloc_globals (genv_genv g) (eval_mem stm) global_definitions with
        | None => True
        | Some m' => m' = m
-       end).
+       end)
+.
 
 (* [match_arg] relates the Coq arguments and the C arguments *)
 Definition match_arg_list : DList.t (fun x => coqType x -> Memory.Mem.mem -> val -> Prop) Args :=
-  args_binary_val64_correct.
+  args_start_addr_correct.
 
 (* [match_res] relates the Coq result and the C result *)
 Definition match_res : coqType Res -> Memory.Mem.mem -> val -> Prop := val64_correct.
@@ -69,13 +73,21 @@ Proof.
   simpl. auto.
 Qed.
 
-Lemma correct_function_addl : correct_function p Args Res f fn match_mem match_arg_list match_res.
+(** How to tell compcert this relation *)
+Axiom id_assum: __1004 = IdentDef.mem_region_id.
+
+Lemma correct_function_start_addr : correct_function p Args Res f fn match_mem match_arg_list match_res.
 Proof.
-  constructor.
+  constructor. (*
   - reflexivity.
   - reflexivity.
-  - reflexivity.
-  - reflexivity.
+  - unfold Args.
+    simpl.
+    unfold mem_region_type.
+    unfold Clightdefs.tptr.
+    rewrite id_assum.
+    reflexivity.
+  - reflexivity.*)
   - unfold Args.
     intro.
     car_cdr.
@@ -85,16 +97,14 @@ Proof.
     (** Here, we know that v = Val.addl (fst c) (fst c0) and m' = m and the trace is empty*)
     (* We need to do it early or we have problems with existentials *)
     destruct c as (v,v').
-    destruct c0 as (c0,c0').
-    unfold val64_correct in *.
+    unfold start_addr_correct in *.
     simpl in H.
-    intuition subst. destruct H3 ; subst.
-    destruct H5 ; subst.
+    intuition subst. clear H2. destruct H1 ; subst. destruct H as [ofs [v'0 [H [H1 H2]]]].
     simpl.
     eexists. eexists. eexists.
     repeat split.
     (* We need to run the program. Some automation is probably possible *)
-    unfold step1.
+    unfold step2.
     apply Smallstep.plus_star.
     eapply Smallstep.plus_left';eauto.
     econstructor ; eauto.
@@ -111,12 +121,56 @@ Proof.
       simpl. intuition congruence.
     + repeat econstructor; eauto.
     + reflexivity.
-    +  eapply Smallstep.plus_one.
+    + eapply Smallstep.plus_one.
       econstructor; eauto.
+      * econstructor;eauto.
+        econstructor;eauto.
+        econstructor;eauto.
+        econstructor;eauto.
+        econstructor;eauto.
+        simpl. rewrite H; reflexivity.
+        simpl.
+        apply deref_loc_copy.
+        simpl; reflexivity.
+        simpl.
+        reflexivity.
+        reflexivity.
+        reflexivity.
+        simpl.
+        econstructor;eauto.
+        simpl.
+        reflexivity.
+        Transparent Archi.align_int64.
+        unfold Archi.align_int64.
+        unfold Coqlib.align.
+        simpl.
+        rewrite Integers.Ptrofs.add_zero.
+        rewrite H in H1.
+        unfold Mem.loadv in H1; simpl in H1.
+        eauto.
+      * simpl.
+        rewrite <- H2.
+        Transparent Archi.ptr64.
+        reflexivity.
+      * 
+        compute.
+        destruct v.
+        simpl in *.
+        
+        unfold Cop.sem_cast.
+         econstructor;eauto.
+        eapply Mem.valid_access_load.
+        *** econstructor;eauto. econstructor;eauto. econstructor;eauto. rewrite Maps.PTree.gss. rewrite H; reflexivity. simpl. Locate deref_loc. constructor. simpl.
+      rewrite H; reflexivity.
        (* We evaluate the expresssions *)
-      econstructor;eauto.
-      econstructor;eauto.
+      repeat econstructor;eauto.
+      rewrite Maps.PTree.gss.
+      rewrite H; reflexivity.
+      simpl.
       reflexivity.
+      econstructor;eauto.
+      econstructor;eauto.
+      econstructor;eauto.
       econstructor;eauto.
       reflexivity.
       Transparent Archi.ptr64.
@@ -126,3 +180,5 @@ Proof.
     + unfold match_mem in H0. destruct H0 as [H0 H1]. assumption.
     + eexists;reflexivity.
 Qed.
+
+End GetMemRegion_start_addr.
